RoboChart/examples/RoboChart_ChemicalDetector_autonomous/RoboChart_Simulation.thy
@@ -29,7 +29,7 @@ removeSubstr w "" = "";
 removeSubstr w s@(c:cs) = (if w `isPrefixOf` s then Prelude.drop (Prelude.length w) s else c : removeSubstr w cs);
 
 replace :: String -> String -> String -> String;
-replace old new = Data.List.intercalate new . Data.List.Split.splitOn old
+replace old new = Data.List.intercalate new . Data.List.Split.splitOn old;
 
 renameGasEvent :: String -> String;
 renameGasEvent gas = 
